src/Lists.v
@@ -2,4 +2,5 @@ Require Export List.
 Require Export FFJ.Lists.Forall2.
 Require Export FFJ.Lists.In.
 Require Export FFJ.Lists.Nth_error.
+Require Export FFJ.Lists.Last_error.
 Require Export FFJ.Lists.ZipWith.
