src/Lists/Last_error.v
@@ -1,0 +1,6 @@
+Require Import List.
+Require Import Tactics.
+Import ListNotations.
+
+Definition last_error {A:Type} (l: list A) :=
+  head (rev (l)).
